TypePM.lean
@@ -3,6 +3,7 @@ import TypePM.Term
 import TypePM.Substitution
 import TypePM.PolySyntax
 import TypePM.PolyScheme
+import TypePM.PolyGeneralization
 import TypePM.PolyInstantiation
 import TypePM.PolyFreshInstantiation
 import TypePM.Relation
